extracted_code/TestProgramSemantics.ml
@@ -1,6 +1,6 @@
 let programs = Shim.listify_coq_list TestPrograms.test_programs
 let get_program = Stdlib.List.nth programs
-let init_state n = CrVarLike.init_concrete_state (get_program n)
+let init_state n = CrVarLike.init_concrete_transformer_state (get_program n)
 let run pid setup =
   let s  = setup (init_state pid) in
   Shim.print_malformed_prog (get_program pid) pid;
