CrConcreteSemanticsTransformer.v
@@ -20,7 +20,7 @@ Definition apply_bin_op (f : BinaryOp) (arg1 : CrVal) (arg2 : CrVal) : CrVal :=
   | ModOp => CrVal.modu arg1 arg2
   end.
 
-Definition lookup_concrete (arg : Operand) (ps : ConcreteState) : CrVal :=
+Definition lookup_concrete (arg : Operand) (ps : ConcreteTransformerState) : CrVal :=
   match arg with
   | OpCtrlPlane c => lookup_varlike_map (@map_from_ps Ctrl _ _ ps) c
   | OpHeader h    => lookup_varlike_map (@map_from_ps Header _ _ ps) h
@@ -37,7 +37,7 @@ Definition apply_bin_op_of (f : BinaryOp) (ty : CrIntType) (v1 v2 : CrVal) : CrV
 Definition apply_cast (from to : CrIntType) (v : CrVal) : CrVal :=
   coerce_to_type to (coerce_to_type from v).
 
-Definition eval_hdr_op_expr_concrete (op : HdrOp) (ps : ConcreteState) : CrVal :=
+Definition eval_hdr_op_expr_concrete (op : HdrOp) (ps : ConcreteTransformerState) : CrVal :=
   match op with
   | StatefulOp f ty arg1 arg2 _ => apply_bin_op_of f ty (lookup_concrete arg1 ps) (lookup_concrete arg2 ps)
   | StatelessOp f ty arg1 arg2 _ => apply_bin_op_of f ty (lookup_concrete arg1 ps) (lookup_concrete arg2 ps)
@@ -45,7 +45,7 @@ Definition eval_hdr_op_expr_concrete (op : HdrOp) (ps : ConcreteState) : CrVal :
   | CastHeaderOp from to arg _ => apply_cast from to (lookup_concrete arg ps)
   end.
 
-Definition eval_hdr_op_assign_concrete (op : HdrOp) (ps: ConcreteState) : ConcreteState :=
+Definition eval_hdr_op_assign_concrete (op : HdrOp) (ps: ConcreteTransformerState) : ConcreteTransformerState :=
   match op with
   | StatefulOp _ _ _ _ target =>
         let op_output := eval_hdr_op_expr_concrete op ps in update_varlike ps target op_output
@@ -64,7 +64,7 @@ Definition eval_cmp_concrete (op : CmpOp) (v1 v2 : CrVal) : bool :=
   | CmpLt => CrVal.ltb v1 v2
   end.
 
-Definition eval_match_concrete (match_pattern : MatchPattern) (ps : ConcreteState) : bool :=
+Definition eval_match_concrete (match_pattern : MatchPattern) (ps : ConcreteTransformerState) : bool :=
   List.forallb (fun '(h, c, v) =>
   let v' := match v with
   | MatchConst k' => (IntVal k')
@@ -74,15 +74,15 @@ Definition eval_match_concrete (match_pattern : MatchPattern) (ps : ConcreteStat
 
 (* Define evaluation over a list of HdrOp *)
 (* The list is evaluated left to right: the head of the list executes first. *)
-Definition eval_hdr_op_list_concrete (hol : list HdrOp) (ps : ConcreteState) : ConcreteState :=
+Definition eval_hdr_op_list_concrete (hol : list HdrOp) (ps : ConcreteTransformerState) : ConcreteTransformerState :=
   List.fold_left (fun acc op => eval_hdr_op_assign_concrete op acc) hol ps.
 
 (* Evalaute a single HdrOp conditionally based on a match_pattern *)
 Definition eval_hdr_op_assign_concrete_conditional
   (match_pattern : MatchPattern)
   (ho : HdrOp)
-  (ps : ConcreteState)
-  : ConcreteState :=
+  (ps : ConcreteTransformerState)
+  : ConcreteTransformerState :=
   if eval_match_concrete match_pattern ps then
     eval_hdr_op_assign_concrete ho ps
   else
@@ -90,7 +90,7 @@ Definition eval_hdr_op_assign_concrete_conditional
  
 (* Function to evaluate a sequential match-action rule,
    meaning header ops within an action are evaluated sequentially *)
-Definition eval_seq_rule_concrete (srule : SeqRule) (ps : ConcreteState) : (ConcreteState) :=
+Definition eval_seq_rule_concrete (srule : SeqRule) (ps : ConcreteTransformerState) : (ConcreteTransformerState) :=
   match srule with
   | SeqCtr match_pattern action =>
       if (eval_match_concrete match_pattern ps) then
@@ -104,7 +104,7 @@ Definition eval_seq_rule_concrete (srule : SeqRule) (ps : ConcreteState) : (Conc
 (* This is identical to eval_seq_rule,
    except that the action is a list with some conditions: the targets are all unique
    these conditions are realized using subset types, that's why we need proj1_sig *)
-Definition eval_par_rule_concrete (prule : ParRule) (ps : ConcreteState) : (ConcreteState) :=
+Definition eval_par_rule_concrete (prule : ParRule) (ps : ConcreteTransformerState) : (ConcreteTransformerState) :=
   match prule with
   | ParCtr match_pattern action =>
       if (eval_match_concrete match_pattern ps) then
@@ -116,14 +116,14 @@ Definition eval_par_rule_concrete (prule : ParRule) (ps : ConcreteState) : (Conc
 (* Function to evaluate a match-action rule,
    meaning header ops within an action are evaluated
    according to the type of the rule (sequential or parallel) *)
-Definition eval_match_action_rule_concrete (rule : MatchActionRule) (ps : ConcreteState) : (ConcreteState) :=
+Definition eval_match_action_rule_concrete (rule : MatchActionRule) (ps : ConcreteTransformerState) : (ConcreteTransformerState) :=
   match rule with 
   | Seq srule => eval_seq_rule_concrete srule ps
   | Par prule => eval_par_rule_concrete prule ps
   end.
 
 (* lookup header against each of the match-action rules in t to see if there is a match *)
-Definition get_match_results (t : Transformer) (ps : ConcreteState) : list bool :=
+Definition get_match_results (t : Transformer) (ps : ConcreteTransformerState) : list bool :=
   List.map (fun rule =>
                      match rule with
                        | Seq (SeqCtr match_pattern _) =>
@@ -133,7 +133,7 @@ Definition get_match_results (t : Transformer) (ps : ConcreteState) : list bool 
                      end) t.
 
 (* Function to evaluate a transformer, which is a list of match-action rules *)
-Definition eval_transformer_concrete (t : Transformer) (ps : ConcreteState) : (ConcreteState) :=
+Definition eval_transformer_concrete (t : Transformer) (ps : ConcreteTransformerState) : (ConcreteTransformerState) :=
     (* Combine match results with the rules to find the first matching rule *)
     let rules_with_match_results := List.combine (get_match_results t ps) t in
     let first_match := find_first_match rules_with_match_results in (* find_first_match is in ListUtils *)
@@ -143,7 +143,7 @@ Definition eval_transformer_concrete (t : Transformer) (ps : ConcreteState) : (C
       end.
 
 (* Function to evaluate a Caracara program *)
-Definition eval_cr_program_concrete (p : CaracaraProgram) (ps : ConcreteState) : (ConcreteState) :=
+Definition eval_cr_program_concrete (p : CaracaraProgram) (ps : ConcreteTransformerState) : (ConcreteTransformerState) :=
   match p with
   | CaracaraProgramDef _ _ _ t => eval_transformer_concrete t ps
   (* TODO: Maybe do something with the various lists of headers, states, and ctrls *)
