CrVarLike.v
@@ -6,6 +6,7 @@ From MyProject Require Import MyInts.
 From MyProject Require Import CrIdentifiers.
 From MyProject Require Import CrProgramState.
 From MyProject Require Import CrModule.
+From MyProject Require Import CrGeneralProgramState.
 From MyProject Require Import CrTransformer.
 From MyProject Require Import SmtExpr.
 From MyProject Require Import CrDsl.
@@ -20,20 +21,20 @@ Import ListNotations.
 Definition injective_contravariant {A B} (f : A -> B) : Prop :=
   forall x y, x <> y -> f x <> f y.
 
-Definition program_state_mapper {T1 T2 : Type} (fc: T1 -> T2) (fh : T1 -> T2) (fs : T1 -> T2) (s: ProgramState T1) : ProgramState T2 :=
-  {| ctrl_map := PMap.map fc (ctrl_map s);
-     header_map := PMap.map fh (header_map s);
-     state_map := PMap.map fs (state_map s) |}.
+Definition program_state_mapper {T1 T2 : Type} (fc: T1 -> T2) (fh : T1 -> T2) (fs : T1 -> T2) (s: TransformerState T1) : TransformerState T2 :=
+  {| t_ctrl_map := PMap.map fc (t_ctrl_map s);
+     t_header_map := PMap.map fh (t_header_map s);
+     t_state_map := PMap.map fs (t_state_map s) |}.
 
 Class CrVarLike (A : Type) := {
   make_item : positive -> A;
   get_key   : A -> positive;
-  map_from_ps : forall {T}, (ProgramState T) -> PMap.t T;
+  map_from_ps : forall {T}, (TransformerState T) -> PMap.t T;
   lookup_varlike_map : forall {T}, PMap.t T -> A -> T := fun {T} m x => PMap.get (get_key x) m;
-  lookup_varlike : forall {T}, (ProgramState T) -> A -> T := fun {T} s x => lookup_varlike_map (map_from_ps s) x;
-  update_all_varlike : forall {T}, (ProgramState T) -> (A -> T) -> ProgramState T;
-  update_varlike : forall {T}, (ProgramState T) -> A -> T -> ProgramState T;
-  is_varlike_in_ps : forall {T}, (ProgramState T) -> A -> option T := fun {T} s v => PTree.get (get_key v) (snd (map_from_ps s));
+  lookup_varlike : forall {T}, (TransformerState T) -> A -> T := fun {T} s x => lookup_varlike_map (map_from_ps s) x;
+  update_all_varlike : forall {T}, (TransformerState T) -> (A -> T) -> TransformerState T;
+  update_varlike : forall {T}, (TransformerState T) -> A -> T -> TransformerState T;
+  is_varlike_in_ps : forall {T}, (TransformerState T) -> A -> option T := fun {T} s v => PTree.get (get_key v) (snd (map_from_ps s));
 
   (* Simple Lemmas *)
   inverses : forall (x : A), make_item (get_key x) = x;
@@ -42,7 +43,7 @@ Class CrVarLike (A : Type) := {
 
   (* Harder lemmas *)
   update_all_varlike_lookup_unchanged :
-  forall {T} (s1 : ProgramState T),
+  forall {T} (s1 : TransformerState T),
   update_all_varlike s1 (fun v : A => lookup_varlike_map (map_from_ps s1) v) = s1;
 
   commute_lookup_varlike:
@@ -54,20 +55,20 @@ Class CrVarLike (A : Type) := {
   program_state_mapper func func func (update_varlike ps x v) = update_varlike (program_state_mapper func func func ps) x (func v);
 
   lookup_varlike_after_update_all_varlike:
-  forall {T} (s1 : ProgramState T) (v : A) (fv : A -> T),
+  forall {T} (s1 : TransformerState T) (v : A) (fv : A -> T),
     is_varlike_in_ps s1 v <> None ->
     lookup_varlike_map (map_from_ps (update_all_varlike s1 fv)) v = fv v;
 }.
 
 Class CrVarLikePairLemmas (A A' : Type) `(CrVarLike A) `(CrVarLike A') := {
   commute_varlike_updates:
-  forall {T} (s1 : ProgramState T)
+  forall {T} (s1 : TransformerState T)
     (fv : A -> T) (fv' : A' -> T),
     update_all_varlike (update_all_varlike s1 fv') fv =
     update_all_varlike (update_all_varlike s1 fv) fv';
 
   is_v1_in_ps_after_update_all_v2:
-  forall {T} (s1 : ProgramState T)
+  forall {T} (s1 : TransformerState T)
     (h : A) (fs : A' -> T),
     is_varlike_in_ps (update_all_varlike s1 fs) h = is_varlike_in_ps s1 h;
 }.
@@ -135,34 +136,34 @@ Instance CrVarLike_Header : CrVarLike Header.
 Proof.
   refine {| make_item := fun uid => HeaderCtr uid;
             get_key := fun h => match h with HeaderCtr uid => uid end;
-            map_from_ps := fun (T : Type) (ps : ProgramState T) => header_map ps;
-            update_all_varlike := fun (T : Type) (ps : ProgramState T) (fh : Header -> T) =>
-              let new_map := new_pmap_from_old (header_map ps) (fun pos => fh (HeaderCtr pos)) in
-              {| ctrl_map := ctrl_map ps;
-                 header_map := new_map;
-                 state_map := state_map ps |};
-            update_varlike := fun (T : Type) (ps : ProgramState T) (h : Header) (v : T) =>
-              let new_map := PMap.set (match h with HeaderCtr uid => uid end) v (header_map ps) in
-              {| ctrl_map := ctrl_map ps;
-                 header_map := new_map;
-                 state_map := state_map ps |}; |}.
+            map_from_ps := fun (T : Type) (ps : TransformerState T) => t_header_map ps;
+            update_all_varlike := fun (T : Type) (ps : TransformerState T) (fh : Header -> T) =>
+              let new_map := new_pmap_from_old (t_header_map ps) (fun pos => fh (HeaderCtr pos)) in
+              {| t_ctrl_map := t_ctrl_map ps;
+                 t_header_map := new_map;
+                 t_state_map := t_state_map ps |};
+            update_varlike := fun (T : Type) (ps : TransformerState T) (h : Header) (v : T) =>
+              let new_map := PMap.set (match h with HeaderCtr uid => uid end) v (t_header_map ps) in
+              {| t_ctrl_map := t_ctrl_map ps;
+                 t_header_map := new_map;
+                 t_state_map := t_state_map ps |}; |}.
   - (* inverses : forall x, make_item (get_key x) = x *)
     intros [uid]. simpl. reflexivity.
   - (* inverses' : forall i, get_key (make_item i) = i *)
     reflexivity.
   - (* inj : injective_contravariant get_key *)
     prove_inj.
-  - (* update_all_varlike_lookup_unchanged : forall {T} (s1 : ProgramState T), update_all_varlike s1 (fun v : A => lookup_varlike_map (map_from_ps s1) v) = s1; *)
+  - (* update_all_varlike_lookup_unchanged : forall {T} (s1 : TransformerState T), update_all_varlike s1 (fun v : A => lookup_varlike_map (map_from_ps s1) v) = s1; *)
     prove_update_all_varlike_lookup_unchanged hdr.
   - (* commute_lookup_varlike:
-      forall {T1 T2} (ps : ProgramState T1) (v : A) (func : T1 -> T2), lookup_varlike (program_state_mapper func func func ps) v = func (lookup_varlike_map (map_from_ps ps) v); *)
+      forall {T1 T2} (ps : TransformerState T1) (v : A) (func : T1 -> T2), lookup_varlike (program_state_mapper func func func ps) v = func (lookup_varlike_map (map_from_ps ps) v); *)
     intros. apply PMap.gmap.
   - (* commute_mapper_update_varlike:
-      forall {T1 T2} (ps : ProgramState T1) (x : A) (v : T1) (func : T1 -> T2),
+      forall {T1 T2} (ps : TransformerState T1) (x : A) (v : T1) (func : T1 -> T2),
       program_state_mapper func func func (update_varlike ps x v) = update_varlike (program_state_mapper func func func ps) x (func v) *)
     prove_commute_mapper_update_varlike.
   - (* lookup_varlike_after_update_all_varlike:
-      forall {T} (s1 : ProgramState T) (v : A) (fv : A -> T),
+      forall {T} (s1 : TransformerState T) (v : A) (fv : A -> T),
         is_varlike_in_ps s1 v <> None ->
         lookup_varlike_map (map_from_ps (update_all_varlike s1 fv)) v = fv v; *)
     prove_lookup_varlike_after_update_all_varlike.
@@ -172,17 +173,17 @@ Instance CrVarLike_State : CrVarLike State.
 Proof.
   refine {| make_item := fun uid => StateCtr uid;
             get_key := fun s => match s with StateCtr uid => uid end;
-            map_from_ps := fun (T : Type) (ps : ProgramState T) => state_map ps;
-            update_all_varlike := fun (T : Type) (ps : ProgramState T) (fs : State -> T) =>
-              let new_map := new_pmap_from_old (state_map ps) (fun pos => fs (StateCtr pos)) in
-              {| ctrl_map := ctrl_map ps;
-                 header_map := header_map ps;
-                 state_map := new_map |};
-            update_varlike := fun (T : Type) (ps : ProgramState T) (h : State) (v : T) =>
-              let new_map := PMap.set (match h with StateCtr uid => uid end) v (state_map ps) in
-              {| ctrl_map := ctrl_map ps;
-                 header_map := header_map ps;
-                 state_map := new_map |}; |}.
+            map_from_ps := fun (T : Type) (ps : TransformerState T) => t_state_map ps;
+            update_all_varlike := fun (T : Type) (ps : TransformerState T) (fs : State -> T) =>
+              let new_map := new_pmap_from_old (t_state_map ps) (fun pos => fs (StateCtr pos)) in
+              {| t_ctrl_map := t_ctrl_map ps;
+                 t_header_map := t_header_map ps;
+                 t_state_map := new_map |};
+            update_varlike := fun (T : Type) (ps : TransformerState T) (h : State) (v : T) =>
+              let new_map := PMap.set (match h with StateCtr uid => uid end) v (t_state_map ps) in
+              {| t_ctrl_map := t_ctrl_map ps;
+                 t_header_map := t_header_map ps;
+                 t_state_map := new_map |}; |}.
   - intros [uid]. simpl. reflexivity.
   - reflexivity.
   - prove_inj.
@@ -196,17 +197,17 @@ Instance CrVarLike_Ctrl : CrVarLike Ctrl.
 Proof.
   refine {| make_item := fun uid => CtrlCtr uid;
             get_key := fun s => match s with CtrlCtr uid => uid end;
-            map_from_ps := fun (T : Type) (ps : ProgramState T) => ctrl_map ps;
-            update_all_varlike := fun (T : Type) (ps : ProgramState T) (fs : Ctrl -> T) =>
-              let new_map := new_pmap_from_old (ctrl_map ps) (fun pos => fs (CtrlCtr pos)) in
-              {| ctrl_map := new_map;
-                 header_map := header_map ps;
-                 state_map := state_map ps |};
-            update_varlike := fun (T : Type) (ps : ProgramState T) (h : Ctrl) (v : T) =>
-              let new_map := PMap.set (match h with CtrlCtr uid => uid end) v (ctrl_map ps) in
-              {| ctrl_map := new_map;
-                 header_map := header_map ps;
-                 state_map := state_map ps |}; |}.
+            map_from_ps := fun (T : Type) (ps : TransformerState T) => t_ctrl_map ps;
+            update_all_varlike := fun (T : Type) (ps : TransformerState T) (fs : Ctrl -> T) =>
+              let new_map := new_pmap_from_old (t_ctrl_map ps) (fun pos => fs (CtrlCtr pos)) in
+              {| t_ctrl_map := new_map;
+                 t_header_map := t_header_map ps;
+                 t_state_map := t_state_map ps |};
+            update_varlike := fun (T : Type) (ps : TransformerState T) (h : Ctrl) (v : T) =>
+              let new_map := PMap.set (match h with CtrlCtr uid => uid end) v (t_ctrl_map ps) in
+              {| t_ctrl_map := new_map;
+                 t_header_map := t_header_map ps;
+                 t_state_map := t_state_map ps |}; |}.
   - intros [uid]. simpl. reflexivity.
   - reflexivity.
   - prove_inj.
@@ -287,10 +288,10 @@ Proof.
 Defined.
 
 Lemma program_state_equality:
-      forall (ps1 ps2: ConcreteState),
-        ctrl_map ps1 = ctrl_map ps2 ->
-        header_map ps1 = header_map ps2 ->
-        state_map  ps1 = state_map ps2 ->
+      forall (ps1 ps2: ConcreteTransformerState),
+        t_ctrl_map ps1 = t_ctrl_map ps2 ->
+        t_header_map ps1 = t_header_map ps2 ->
+        t_state_map  ps1 = t_state_map ps2 ->
         ps1 = ps2.
 Proof.
   intros ps1 ps2 Hctrl Hhdr Hstate.
@@ -301,7 +302,7 @@ Proof.
 Qed.
 
 Lemma program_state_unchanged:
-  forall {T} (s1 : ProgramState T),
+  forall {T} (s1 : TransformerState T),
   update_all_varlike (update_all_varlike s1 (fun h : Header => lookup_varlike_map ((@map_from_ps Header CrVarLike_Header T) s1) h))
                     (fun s : State => lookup_varlike_map ((@map_from_ps State CrVarLike_State T) s1) s) = s1.
 Proof.
@@ -341,12 +342,12 @@ Proof.
   intros [i] [j] _ _ Hneq Heq. simpl in Heq. subst. apply Hneq. reflexivity.
 Qed.
 
-Definition get_all_varlike_from_ps {T A : Type} `{CrVarLike A} (s: ProgramState T) : list A :=
+Definition get_all_varlike_from_ps {T A : Type} `{CrVarLike A} (s: TransformerState T) : list A :=
   List.map (fun '(key, value) => make_item key)
            (PTree.elements (snd (map_from_ps s))).
 
 Lemma is_varlike_in_ps_lemma :
-  forall {T A} `{CrVarLike A} (s1 : ProgramState T) (v : A),
+  forall {T A} `{CrVarLike A} (s1 : TransformerState T) (v : A),
     In v (get_all_varlike_from_ps s1) ->
     is_varlike_in_ps s1 v <> None.
 Proof.
@@ -355,9 +356,9 @@ Proof.
   unfold get_all_varlike_from_ps in H.
   unfold is_varlike_in_ps.
   simpl in *.
-  destruct ctrl as [c0 ctrl_map].
+  destruct ctrl as [c0 t_ctrl_map].
   destruct hdr as [h0 hdr_map].
-  destruct state as [s0 state_map].
+  destruct state as [s0 t_state_map].
   simpl in *.
   apply in_map_iff in H.
   destruct H. (* TODO: ask Joe, seems to extract witness *)
@@ -369,13 +370,21 @@ Proof.
   assumption.
 Qed.
 
-Definition init_concrete_state (p : CaracaraProgram) : ConcreteState :=
+Definition init_concrete_transformer_state (p : CaracaraProgram) : ConcreteTransformerState :=
   let h := get_headers_from_prog p in
   let s := get_states_from_prog p in
   let c := get_ctrls_from_prog p in
-  {|ctrl_map    :=  PMap.init (IntVal CrNilInt);
-     header_map :=  PMap.init (IntVal CrNilInt);
-     state_map  :=  PMap.init (IntVal CrNilInt);|}.
+  {|t_ctrl_map    :=  PMap.init (IntVal CrNilInt);
+     t_header_map :=  PMap.init (IntVal CrNilInt);
+     t_state_map  :=  PMap.init (IntVal CrNilInt);|}.
+
+(* Concrete initial state for a parser module: an empty header map and an
+   empty input packet (the packet bits are injected at run time).  Mirrors
+   [init_concrete_transformer_state]. *)
+Definition init_concrete_parser_state : ModuleState CrVal bool :=
+  ParserMod {| p_header_map := PMap.init (IntVal CrNilInt);
+               p_packet     := @nil bool;
+               p_cursor     := 0 |}.
 
 (* Convert positive to string *)
 Fixpoint pos_to_string (p : positive) : string :=
@@ -428,47 +437,38 @@ Proof.
 Qed.
 
 Local Open Scope string_scope.
-Definition init_symbolic_state (p: CaracaraProgram) : SymbolicState :=
+Definition init_symbolic_transformer_state (prefix: string) (p: CaracaraProgram) : SymbolicTransformerState :=
   let h := get_headers_from_prog p in
   let s := get_states_from_prog p in
   let c := get_ctrls_from_prog p in
-  {| ctrl_map   :=  (SmtArithConst CrNilInt,
+  {| t_ctrl_map   :=  (SmtArithConst CrNilInt,
                       PTree_Properties.of_list
-                      (List.map (fun x => let var := match x with | CtrlCtr x_id => x_id end in (var,  SmtArithVar ("ctrl_" ++ pos_to_string var))) c));
-     header_map :=  (SmtArithConst CrNilInt,
+                      (List.map (fun x => let x' := unwrap x in (x', SmtArithVar (prefix ++ "ctrl_" ++ pos_to_string x'))) c));
+     t_header_map :=  (SmtArithConst CrNilInt,
                       PTree_Properties.of_list
-                      (List.map (fun x => let var := match x with | HeaderCtr x_id => x_id end in (var, SmtArithVar ("hdr_" ++ pos_to_string var))) h));
-     state_map  :=  (SmtArithConst CrNilInt,
+                      (List.map (fun x => let x' := unwrap x in (x', SmtArithVar ("hdr_" ++ pos_to_string x'))) h));
+     t_state_map  :=  (SmtArithConst CrNilInt,
                       PTree_Properties.of_list
-                      (List.map (fun x => let var := match x with | StateCtr x_id => x_id end in (var, SmtArithVar ("state_" ++ pos_to_string var))) s));|}.
+                      (List.map (fun x => let x' := unwrap x in (x', SmtArithVar (prefix ++ "state_" ++ pos_to_string x'))) s));|}.
+Definition init_symbolic_transformer_state' (p : CaracaraProgram) : SymbolicTransformerState :=
+  init_symbolic_transformer_state "" p.
 
-Definition init_module_symbolic_state
-    (prog_prefix : string)
-    (m_id        : ModuleName)
-    (h           : list Header)
-    (s           : list State)
-    (c           : list Ctrl)
-    : SymbolicState :=
-  (* e.g. p1_m4_ *)
-  let m_prefix := prog_prefix ++ "_m" ++ pos_to_string (unwrap m_id) ++ "_" in
-  {| ctrl_map :=
-       (SmtArithConst CrNilInt,
-        PTree_Properties.of_list
-          (List.map (fun x =>
-            let var := match x with | CtrlCtr x_id => x_id end in
-            (var, SmtArithVar (m_prefix ++ "ctrl_" ++ pos_to_string var))) c));
-     header_map :=
-       (SmtArithConst CrNilInt,
-        PTree_Properties.of_list
-          (List.map (fun x =>
-            let var := match x with | HeaderCtr x_id => x_id end in
-            (var, SmtArithVar ("hdr_" ++ pos_to_string var))) h));
-     state_map :=
-       (SmtArithConst CrNilInt,
-        PTree_Properties.of_list
-          (List.map (fun x =>
-            let var := match x with | StateCtr x_id => x_id end in
-            (var, SmtArithVar (m_prefix ++ "state_" ++ pos_to_string var))) s));|}.
+Definition init_symbolic_parser_state (prefix : string) (h : list Header) : SymbolicParserState :=
+  {| p_header_map := (SmtArithConst CrNilInt,
+                     PTree_Properties.of_list
+                     (List.map (fun x => let x' := unwrap x in (x', SmtArithVar ("hdr_" ++ pos_to_string x'))) h));
+     p_packet := @nil SmtBoolExpr;
+     p_cursor := 0 |}.
+
+Definition init_sym_t_state (prog_prefix : string) (m_id : ModuleName) (p : CaracaraProgram)
+  : SymbolicTransformerState :=
+  let prefix := prog_prefix ++ "_m" ++ pos_to_string (unwrap m_id) ++ "_" in
+  init_symbolic_transformer_state prefix p.
+
+Definition init_sym_p_state (prog_prefix : string) (m_id : ModuleName) (h : list Header)
+  : SymbolicParserState :=
+  let prefix := prog_prefix ++ "_m" ++ pos_to_string (unwrap m_id) ++ "_" in
+  init_symbolic_parser_state prefix h.
 
 Definition collect_write_headers (mods : list CrModule) : list Header :=
   List.flat_map (fun m =>
@@ -490,42 +490,56 @@ Definition init_general_symbolic_state
   let mods := net_modules net in
   let h := get_headers_from_general p in
   let write_hdrs := collect_write_headers mods in
-  List.fold_left
+  let ms := List.fold_left
     (fun acc m =>
       match m with
-      | ParserModule _ _ => acc
+      | ParserModule m_id _ =>
+        let base := init_sym_p_state prog_prefix m_id h in
+        PMap.set (unwrap m_id) (ParserMod base) acc
       | TransformerModule m_id s c t =>
-        let base := init_module_symbolic_state prog_prefix m_id h s c in
+        let local_program := CaracaraProgramDef h s c [] in
+        let base := init_sym_t_state prog_prefix m_id local_program in
         (* Seed each write-target header explicitly in the PTree so that
-           update_all_varlike will track it after eval_transformer_smt runs.
-           For input headers already present this is a no-op; for output-only
-           headers it installs their PMap default (CrNilInt) as an explicit entry. *)
+          update_all_varlike will track it after eval_transformer_smt runs.
+          For input headers already present this is a no-op; for output-only
+          headers it installs their PMap default (CrNilInt) as an explicit entry. *)
         let seeded := List.fold_left
           (fun st wh => update_varlike st wh (lookup_varlike st wh))
           write_hdrs base in
-        PMap.set (unwrap m_id) seeded acc
+        PMap.set (unwrap m_id) (TransformerMod seeded) acc
       end)
     mods
-    (PMap.init {|
-      ctrl_map := PMap.init (SmtArithConst CrNilInt);
-      header_map := PMap.init (SmtArithConst CrNilInt);
-      state_map := PMap.init (SmtArithConst CrNilInt);
-    |}).
+    (PMap.init (TransformerMod {|
+      t_ctrl_map := PMap.init (SmtArithConst CrNilInt);
+      t_header_map := PMap.init (SmtArithConst CrNilInt);
+      t_state_map := PMap.init (SmtArithConst CrNilInt);
+    |})) in
+  (* Shared global header channel: seed with the un-prefixed input header
+     symbolic variables (the shared cross-module/cross-program interface). *)
+  let sh_hdr := p_header_map (init_symbolic_parser_state "" h) in
+  {| sh_hdr_map := sh_hdr;
+     sh_bit_map := @nil SmtBoolExpr;
+     mod_states := ms |}.
 
 Definition init_general_concrete_state (p : GeneralCaracaraProgram)
     : GeneralConcreteState :=
   let net := get_network_from_general p in
-  List.fold_left
+  let ms := List.fold_left
     (fun acc m =>
       match m with
-      | ParserModule _ _ => acc
+      | ParserModule m_id _ =>
+          PMap.set (unwrap m_id) init_concrete_parser_state acc
       | TransformerModule m_id s c _ =>
-          PMap.set (unwrap m_id) (init_concrete_state (CaracaraProgramDef [] s c [])) acc
+          PMap.set (unwrap m_id)
+            (TransformerMod (init_concrete_transformer_state (CaracaraProgramDef [] s c []))) acc
       end)
     (net_modules net)
-    (PMap.init (init_concrete_state (CaracaraProgramDef [] [] [] []))).
+    (PMap.init (TransformerMod (init_concrete_transformer_state (CaracaraProgramDef [] [] [] [])))) in
+  {| sh_hdr_map := PMap.init (IntVal CrNilInt);
+     sh_bit_map := @nil bool;
+     mod_states := ms |}.
 
-Definition is_init_state {T} (p : CaracaraProgram) (ps : ProgramState T) : Prop :=
+Definition is_init_state {T} (p : CaracaraProgram) (ps : TransformerState T) : Prop :=
   forall h sv c,
     (In h (get_headers_from_prog p) <-> In h (get_all_varlike_from_ps ps)) /\
     (In sv (get_states_from_prog p) <-> In sv (get_all_varlike_from_ps ps)) /\
