SmtQuery.v
@@ -22,8 +22,8 @@ Import ListNotations.
 From MyProject Require Import CrTransformer.
 From MyProject Require Import CrSymbolicSemanticsTransformer.
 From MyProject Require Import CrConcreteSemanticsTransformer.
-From MyProject Require Import CrTModSymbolicSemantics.
-From MyProject Require Import CrTModConcreteSemantics.
+From MyProject Require Import CrModSymbolicSemantics.
+From MyProject Require Import CrModConcreteSemantics.
 From MyProject Require Import ConcreteToSymbolicLemmas.
 From MyProject Require Import SmtHelperLemmas.
 From MyProject Require Import UtilLemmas.
@@ -50,7 +50,7 @@ Axiom smt_query_sound_none : forall e,
 (* Need to look at all variables within s1 and s2,
    which means we need to iterate through header_list and state_var_list *)
 (* function that given 2 states and a list of headers and state vars, asserts that each header/state var is the same across the two states *)
-Definition check_headers_and_state_vars (s1 s2 : SymbolicState)
+Definition check_headers_and_state_vars (s1 s2 : SymbolicTransformerState)
   (header_list : list Header) (state_var_list : list State)
   : SmtBoolExpr :=
   SmtBoolNot(
@@ -167,7 +167,7 @@ Proof.
 Qed.
 
 Definition equivalence_checker
-  (s : SymbolicState)
+  (s : SymbolicTransformerState)
   (t1 : Transformer) (t2 : Transformer)
   (header_list : list Header) (state_var_list : list State)
    :  SmtResult :=
@@ -192,7 +192,7 @@ Definition equivalence_checker_cr_dsl (p1: CaracaraProgram) (p2: CaracaraProgram
       if varlike_list_equal h1 h2 then
         if varlike_list_equal s1 s2 then
           if varlike_list_equal c1 c2 then
-            match (equivalence_checker (init_symbolic_state p1) t1 t2 h1 s1) with
+            match (equivalence_checker (init_symbolic_transformer_state' p1) t1 t2 h1 s1) with
             (* TODO: Maybe equivalence_checker should take c as argument too? *)
             | SmtUnsat => Equivalent (* if it is unsatisfiable, then all state vars and headers are equal *)
             | SmtSat f => NotEquivalent f (* if it is satisfiable, then some state var or header is not equal *)
@@ -292,17 +292,18 @@ Proof.
 Qed.
 
 Lemma init_symbolic_state_nodep_t : forall h s c t1 t2,
-  init_symbolic_state (CaracaraProgramDef h s c t1) =
-  init_symbolic_state (CaracaraProgramDef h s c t2).
+  init_symbolic_transformer_state' (CaracaraProgramDef h s c t1) =
+  init_symbolic_transformer_state' (CaracaraProgramDef h s c t2).
 Proof.
   intros h s c t1 t2.
-  unfold init_symbolic_state.
+  unfold init_symbolic_transformer_state',
+         init_symbolic_transformer_state.
   f_equal.
 Qed.
 
 Class CrVarProg A := {
   get_vars_from_prog : CaracaraProgram -> list A;
-  lookup_var : ConcreteState -> A -> CrVal;
+  lookup_var : ConcreteTransformerState -> A -> CrVal;
   get_vars_invariant_of_transformer:
     forall h s c t1 t2,
     get_vars_from_prog (CaracaraProgramDef h s c t1) =
@@ -311,8 +312,8 @@ Class CrVarProg A := {
     forall p1 p2 f,
     well_formed_program p1 ->                          (* p1 is well-formed *)
     equivalence_checker_cr_dsl p1 p2 = Equivalent ->
-    let c1_i  := eval_sym_state (init_symbolic_state p1) f in (* Get a sym state out of p1 *)
-    let c2_i  := eval_sym_state (init_symbolic_state p2) f in (* Do the same for p2 *)
+    let c1_i  := eval_sym_state (init_symbolic_transformer_state' p1) f in (* Get a sym state out of p1 *)
+    let c2_i  := eval_sym_state (init_symbolic_transformer_state' p2) f in (* Do the same for p2 *)
     let t1 := get_transformer_from_prog p1 in
     let t2 := get_transformer_from_prog p2 in
     let c1 := eval_transformer_concrete t1 c1_i in
@@ -325,7 +326,8 @@ Class CrVarProg A := {
 Ltac prove_in_var_list_implies_in_prog_state hypothesis type crvar_type :=
   intros;
   apply is_varlike_in_ps_lemma;
-  unfold init_symbolic_state;
+  unfold init_symbolic_transformer_state',
+         init_symbolic_transformer_state;
   unfold get_all_varlike_from_ps;
   simpl;
   repeat rewrite map_pair_split;
@@ -351,7 +353,7 @@ Ltac prove_equivalence_checker_cr_sound :=
   simpl in H1;
   split;
   try (rewrite H_hdr_eq in H1; assumption); try (rewrite H_state_eq in H1; assumption);
-  destruct (equivalence_checker (init_symbolic_state (CaracaraProgramDef h1 s1 c1 t1)) t1 t2 h1 s1) eqn:H_eq; try (exfalso; congruence);
+  destruct (equivalence_checker (init_symbolic_transformer_state' (CaracaraProgramDef h1 s1 c1 t1)) t1 t2 h1 s1) eqn:H_eq; try (exfalso; congruence);
   apply equivalence_checker_sound with (f := f) in H_eq;
   try(apply H_eq in H1;
       unfold c0, c3, c1_i, c2_i, t0, t3;
@@ -396,13 +398,13 @@ Lemma equivalence_checker_cr_complete :
   well_formed_program p1 ->                          (* p1 is well-formed *)
   well_formed_program p2 ->                          (* p2 is well-formed *)
   equivalence_checker_cr_dsl p1 p2 = NotEquivalent f ->
-  let c1_i  := eval_sym_state (init_symbolic_state p1) f in (* Get a sym state out of p1' headers, ctrls, and state *)
-  let c2_i  := eval_sym_state (init_symbolic_state p2) f in (* Do the same for p2 *)
+  let c1_i  := eval_sym_state (init_symbolic_transformer_state' p1) f in (* Get a sym state out of p1' headers, ctrls, and state *)
+  let c2_i  := eval_sym_state (init_symbolic_transformer_state' p2) f in (* Do the same for p2 *)
   let t1 := get_transformer_from_prog p1 in
   let t2 := get_transformer_from_prog p2 in
   let c1 := eval_transformer_concrete t1 c1_i in
   let c2 := eval_transformer_concrete t2 c2_i in
-  (init_symbolic_state p1 = init_symbolic_state p2) ->  (* both programs have the same initial symbolic state
+  (init_symbolic_transformer_state' p1 = init_symbolic_transformer_state' p2) ->  (* both programs have the same initial symbolic state
                                                            , i.e., same headers, ctrls, and states *)
                                                            (* TODO handle case where programs
                                                            are not equivalent bcos headers, ctrls, and states differ *)
@@ -419,13 +421,13 @@ Proof.
   (varlike_list_equal s1 s2) eqn:H_state_eq,
   (varlike_list_equal c1 c2) eqn:H_ctrl_eq in H; simpl in H.
   2-8: discriminate H. (* The easy goals, where state, ctrl, or header lists are NOT equal, proof by explosion because we assume these lists ARE equal*)
-  - destruct (equivalence_checker (init_symbolic_state (CaracaraProgramDef h1 s1 c1 (* The hard goal *)
+  - destruct (equivalence_checker (init_symbolic_transformer_state' (CaracaraProgramDef h1 s1 c1 (* The hard goal *)
 t1)) t1 t2 h1 s1) eqn:H_eq; try (exfalso; congruence).
     -- simpl.
        intros.
        apply equivalence_checker_complete
         with (f' := f0)
-             (s := init_symbolic_state (CaracaraProgramDef h1 s1 c1 t1)) 
+             (s := init_symbolic_transformer_state' (CaracaraProgramDef h1 s1 c1 t1)) 
              (header_list := h1) (state_var_list := s1) in H_eq.
        ++ simpl.
           injection H as Heq.
@@ -477,12 +479,12 @@ Definition map_is_valid (m : PMap.t CrVal) : Prop :=
 
 (* A concrete state cs is valid relative to a program p when:
    - each PMap has (IntVal CrNilInt) as its default,
-   - every value in cs is either (IntVal CrNilInt) or a uint8, and
+   - every value in cs is either (IntVal CrNilInt) or an (IntVal (CrInt _)), and
    - the initialized variables in cs are exactly the program variables of p. *)
-Definition concrete_state_is_valid (p : CaracaraProgram) (cs : ConcreteState) : Prop :=
-  map_is_valid (header_map cs) /\
-  map_is_valid (state_map cs) /\
-  map_is_valid (ctrl_map cs) /\
+Definition concrete_state_is_valid (p : CaracaraProgram) (cs : ConcreteTransformerState) : Prop :=
+  map_is_valid (t_header_map cs) /\
+  map_is_valid (t_state_map cs) /\
+  map_is_valid (t_ctrl_map cs) /\
   (forall v : Header, lookup_varlike cs v <> (IntVal CrNilInt) <-> In v (get_headers_from_prog p)) /\
   (forall v : State,  lookup_varlike cs v <> (IntVal CrNilInt) <-> In v (get_states_from_prog p)) /\
   (forall v : Ctrl,   lookup_varlike cs v <> (IntVal CrNilInt) <-> In v (get_ctrls_from_prog p)).
@@ -536,22 +538,22 @@ Proof.
     + exact IH.
 Qed.
 
-Definition build_valuation_for_cs (cs : ConcreteState) : SmtValuation :=
+Definition build_valuation_for_cs (cs : ConcreteTransformerState) : SmtValuation :=
   fun name =>
-    match try_match_prefix "hdr_" (PTree.elements (snd (header_map cs))) name with
+    match try_match_prefix "hdr_" (PTree.elements (snd (t_header_map cs))) name with
     | Some v => v
     | None =>
-      match try_match_prefix "state_" (PTree.elements (snd (state_map cs))) name with
+      match try_match_prefix "state_" (PTree.elements (snd (t_state_map cs))) name with
       | Some v => v
       | None =>
-        match try_match_prefix "ctrl_" (PTree.elements (snd (ctrl_map cs))) name with
+        match try_match_prefix "ctrl_" (PTree.elements (snd (t_ctrl_map cs))) name with
         | Some v => v
         | None => IntVal (CrInt (repr 0))
         end
       end
     end.
 
-Local Ltac uint8_finalize valid_lemma id_var :=
+Local Ltac int_value_finalize valid_lemma id_var :=
   pose proof (valid_lemma id_var) as Hvv;
   unfold value_is_valid in Hvv;
   match goal with
@@ -569,7 +571,7 @@ Lemma valid_states_realizable :
   (* there is a valuation f under which init_symbolic_state p concretizes
      to a state that agrees with cs at every variable *)
   exists f,
-  let c := eval_sym_state (init_symbolic_state p) f in
+  let c := eval_sym_state (init_symbolic_transformer_state' p) f in
   (forall (v : Header), lookup_varlike c v = lookup_varlike cs v) /\
   (forall (v : State),  lookup_varlike c v = lookup_varlike cs v) /\
   (forall (v : Ctrl),   lookup_varlike c v = lookup_varlike cs v).
@@ -594,9 +596,9 @@ Proof.
     rewrite lookup_varlike_header_PMap_concrete.
     destruct (List.in_dec posesque_eq_dec (HeaderCtr id) hp) as [Hin | Hnin].
     + (* In p's list: cs is initialized at id, agrees with f *)
-      assert (Hneq : PMap.get id (header_map cs) <> IntVal CrNilInt).
+      assert (Hneq : PMap.get id (t_header_map cs) <> IntVal CrNilInt).
       { apply (proj2 (Hh_in (HeaderCtr id))). assumption. }
-      assert (Htree : (snd (header_map cs)) ! id = Some (PMap.get id (header_map cs))).
+      assert (Htree : (snd (t_header_map cs)) ! id = Some (PMap.get id (t_header_map cs))).
       { eapply cs_initialized_in_tree_header; eauto. }
       rewrite init_sym_header_lookup with (id := id).
       3: { assumption. }
@@ -604,8 +606,8 @@ Proof.
       simpl.
       unfold build_valuation_for_cs.
       rewrite try_match_prefix_found
-        with (id := id) (w := PMap.get id (header_map cs)).
-      * uint8_finalize Hh_valid id.
+        with (id := id) (w := PMap.get id (t_header_map cs)).
+      * int_value_finalize Hh_valid id.
       * apply PTree.elements_keys_norepet.
       * apply PTree.elements_correct. assumption.
     + (* Not in p's list: both sides equal IntVal CrNilInt *)
@@ -615,7 +617,7 @@ Proof.
       pose proof (Hh_in (HeaderCtr id)) as Hiff.
       rewrite lookup_varlike_header_PMap_concrete in Hiff.
       pose proof (Hh_valid id) as Hvv. unfold value_is_valid, PMap.get in *.
-      destruct ((snd (header_map cs)) ! id) as [w|] eqn:Htree.
+      destruct ((snd (t_header_map cs)) ! id) as [w|] eqn:Htree.
       * destruct w as [i| | |]; try contradiction.
         destruct i; try contradiction.
         -- exfalso. apply Hnin. apply (proj1 Hiff). discriminate.
@@ -627,9 +629,9 @@ Proof.
     rewrite lookup_varlike_state_PMap.
     rewrite lookup_varlike_state_PMap_concrete.
     destruct (List.in_dec posesque_eq_dec (StateCtr id) sp) as [Hin | Hnin].
-    + assert (Hneq : PMap.get id (state_map cs) <> IntVal CrNilInt).
+    + assert (Hneq : PMap.get id (t_state_map cs) <> IntVal CrNilInt).
       { apply (proj2 (Hs_in (StateCtr id))). assumption. }
-      assert (Htree : (snd (state_map cs)) ! id = Some (PMap.get id (state_map cs))).
+      assert (Htree : (snd (t_state_map cs)) ! id = Some (PMap.get id (t_state_map cs))).
       { eapply cs_initialized_in_tree_state; eauto. }
       rewrite init_sym_state_lookup with (id := id).
       3: { assumption. }
@@ -639,8 +641,8 @@ Proof.
       rewrite try_match_prefix_not_found_diff_char with (c1 := "h"%char) (c2 := "s"%char).
       2: { intros H; inversion H. }
       rewrite try_match_prefix_found
-        with (id := id) (w := PMap.get id (state_map cs)).
-      * uint8_finalize Hs_valid id.
+        with (id := id) (w := PMap.get id (t_state_map cs)).
+      * int_value_finalize Hs_valid id.
       * apply PTree.elements_keys_norepet.
       * apply PTree.elements_correct. assumption.
     + rewrite (init_sym_state_lookup_default (CaracaraProgramDef hp sp cp []) id).
@@ -649,7 +651,7 @@ Proof.
       pose proof (Hs_in (StateCtr id)) as Hiff.
       rewrite lookup_varlike_state_PMap_concrete in Hiff.
       pose proof (Hs_valid id) as Hvv. unfold value_is_valid, PMap.get in *.
-      destruct ((snd (state_map cs)) ! id) as [w|] eqn:Htree.
+      destruct ((snd (t_state_map cs)) ! id) as [w|] eqn:Htree.
       * destruct w as [i| | |]; try contradiction.
         destruct i; try contradiction.
         -- exfalso. apply Hnin. apply (proj1 Hiff). discriminate.
@@ -661,9 +663,9 @@ Proof.
     rewrite lookup_varlike_ctrl_PMap.
     rewrite lookup_varlike_ctrl_PMap_concrete.
     destruct (List.in_dec posesque_eq_dec (CtrlCtr id) cp) as [Hin | Hnin].
-    + assert (Hneq : PMap.get id (ctrl_map cs) <> IntVal CrNilInt).
+    + assert (Hneq : PMap.get id (t_ctrl_map cs) <> IntVal CrNilInt).
       { apply (proj2 (Hc_in (CtrlCtr id))). assumption. }
-      assert (Htree : (snd (ctrl_map cs)) ! id = Some (PMap.get id (ctrl_map cs))).
+      assert (Htree : (snd (t_ctrl_map cs)) ! id = Some (PMap.get id (t_ctrl_map cs))).
       { eapply cs_initialized_in_tree_ctrl; eauto. }
       rewrite init_sym_ctrl_lookup with (id := id).
       3: { assumption. }
@@ -675,8 +677,8 @@ Proof.
       rewrite try_match_prefix_not_found_diff_char with (c1 := "s"%char) (c2 := "c"%char).
       2: { intros H; inversion H. }
       rewrite try_match_prefix_found
-        with (id := id) (w := PMap.get id (ctrl_map cs)).
-      * uint8_finalize Hc_valid id.
+        with (id := id) (w := PMap.get id (t_ctrl_map cs)).
+      * int_value_finalize Hc_valid id.
       * apply PTree.elements_keys_norepet.
       * apply PTree.elements_correct. assumption.
     + rewrite (init_sym_ctrl_lookup_default (CaracaraProgramDef hp sp cp []) id).
@@ -685,7 +687,7 @@ Proof.
       pose proof (Hc_in (CtrlCtr id)) as Hiff.
       rewrite lookup_varlike_ctrl_PMap_concrete in Hiff.
       pose proof (Hc_valid id) as Hvv. unfold value_is_valid, PMap.get in *.
-      destruct ((snd (ctrl_map cs)) ! id) as [w|] eqn:Htree.
+      destruct ((snd (t_ctrl_map cs)) ! id) as [w|] eqn:Htree.
       * destruct w as [i| | |]; try contradiction.
         destruct i; try contradiction.
         -- exfalso. apply Hnin. apply (proj1 Hiff). discriminate.
@@ -699,7 +701,7 @@ Lemma in_program_implies_in_init_sym_header :
   forall p (v : Header),
     well_formed_program p ->
     In v (get_headers_from_prog p) ->
-    is_varlike_in_ps (init_symbolic_state p) v <> None.
+    is_varlike_in_ps (init_symbolic_transformer_state' p) v <> None.
 Proof.
   intros p v Hwf Hin.
   apply is_varlike_in_ps_lemma.
@@ -715,7 +717,7 @@ Lemma in_program_implies_in_init_sym_state :
   forall p (v : State),
     well_formed_program p ->
     In v (get_states_from_prog p) ->
-    is_varlike_in_ps (init_symbolic_state p) v <> None.
+    is_varlike_in_ps (init_symbolic_transformer_state' p) v <> None.
 Proof.
   intros p v Hwf Hin.
   apply is_varlike_in_ps_lemma.
@@ -754,16 +756,16 @@ Proof.
   destruct (varlike_list_equal h1 h2),
            (varlike_list_equal s1 s2),
            (varlike_list_equal c1 c2); try congruence.
-  destruct (equivalence_checker (init_symbolic_state p1) t1 t2 h1 s1) eqn:Heq; try congruence.
+  destruct (equivalence_checker (init_symbolic_transformer_state' p1) t1 t2 h1 s1) eqn:Heq; try congruence.
   clear Heq'.
   unfold equivalence_checker in Heq.
   apply smt_query_sound_none with (v' := f) in Heq.
   apply check_headers_and_state_vars_false in Heq.
   destruct Heq as [Hheq Hseq].
   assert (Hbridge : forall (h : Header) (s : State) (c : Ctrl),
-    lookup_varlike c_init h = lookup_varlike (eval_sym_state (init_symbolic_state p1) f) h /\
-    lookup_varlike c_init s = lookup_varlike (eval_sym_state (init_symbolic_state p1) f) s /\
-    lookup_varlike c_init c = lookup_varlike (eval_sym_state (init_symbolic_state p1) f) c).
+    lookup_varlike c_init h = lookup_varlike (eval_sym_state (init_symbolic_transformer_state' p1) f) h /\
+    lookup_varlike c_init s = lookup_varlike (eval_sym_state (init_symbolic_transformer_state' p1) f) s /\
+    lookup_varlike c_init c = lookup_varlike (eval_sym_state (init_symbolic_transformer_state' p1) f) c).
   { intros h s c. split; [| split].
     - rewrite (Hvsr1_hdrs h). reflexivity.
     - rewrite (Hvsr1_states s). reflexivity.
@@ -775,15 +777,15 @@ Proof.
     specialize (Hheq v Hv).
     apply smt_bool_eq_true in Hheq.
     repeat rewrite commute_conc_and_lookup in Hheq.
-    assert (Hin_ps : is_varlike_in_ps (init_symbolic_state p1) v <> None).
+    assert (Hin_ps : is_varlike_in_ps (init_symbolic_transformer_state' p1) v <> None).
     { apply in_program_implies_in_init_sym_header with (p := p1).
       - exact Hwf1_orig.
       - rewrite desp1. simpl. exact Hv. }
     rewrite <- commute_sym_vs_conc_transformer_header_map
-      with (t := t1) (f := f) (s1 := init_symbolic_state p1) (h := v) in Hheq;
+      with (t := t1) (f := f) (s1 := init_symbolic_transformer_state' p1) (h := v) in Hheq;
       try assumption.
     rewrite <- commute_sym_vs_conc_transformer_header_map
-      with (t := t2) (f := f) (s1 := init_symbolic_state p1) (h := v) in Hheq;
+      with (t := t2) (f := f) (s1 := init_symbolic_transformer_state' p1) (h := v) in Hheq;
       try assumption.
     specialize (Hbridge_t1 v (StateCtr 1) (CtrlCtr 1)) as [Hbt1 _].
     specialize (Hbridge_t2 v (StateCtr 1) (CtrlCtr 1)) as [Hbt2 _].
@@ -793,15 +795,15 @@ Proof.
     specialize (Hseq v Hv).
     apply smt_bool_eq_true in Hseq.
     repeat rewrite commute_conc_and_lookup in Hseq.
-    assert (Hin_ps : is_varlike_in_ps (init_symbolic_state p1) v <> None).
+    assert (Hin_ps : is_varlike_in_ps (init_symbolic_transformer_state' p1) v <> None).
     { apply in_program_implies_in_init_sym_state with (p := p1).
       - exact Hwf1_orig.
       - rewrite desp1. simpl. exact Hv. }
     rewrite <- commute_sym_vs_conc_transformer_state_var_map
-      with (t := t1) (f := f) (s1 := init_symbolic_state p1) (sv := v) in Hseq;
+      with (t := t1) (f := f) (s1 := init_symbolic_transformer_state' p1) (sv := v) in Hseq;
       try assumption.
     rewrite <- commute_sym_vs_conc_transformer_state_var_map
-      with (t := t2) (f := f) (s1 := init_symbolic_state p1) (sv := v) in Hseq;
+      with (t := t2) (f := f) (s1 := init_symbolic_transformer_state' p1) (sv := v) in Hseq;
       try assumption.
     specialize (Hbridge_t1 (HeaderCtr 1) v (CtrlCtr 1)) as [_ [Hbt1 _]].
     specialize (Hbridge_t2 (HeaderCtr 1) v (CtrlCtr 1)) as [_ [Hbt2 _]].
