CrGeneralProgramState.v
@@ -1,0 +1,39 @@
+From MyProject Require Import Maps.
+From MyProject Require Import CrProgramState.
+From MyProject Require Import CrVal.
+From MyProject Require Import SmtExpr.
+
+(* [Th] is the header-value type, [Tb] the packet-bit type. *)
+Record GeneralProgramState (Th Tb : Type) := {
+  sh_hdr_map : PMap.t Th;
+  sh_bit_map : list Tb;
+  mod_states : PMap.t (ModuleState Th Tb);
+}.
+
+Arguments sh_hdr_map {Th Tb} _.
+Arguments sh_bit_map {Th Tb} _.
+Arguments mod_states {Th Tb} _.
+
+Definition set_gps_shared_headers {Th Tb : Type}
+  (gps : GeneralProgramState Th Tb) (hdrs : PMap.t Th)
+  : GeneralProgramState Th Tb :=
+  {| sh_hdr_map := hdrs;
+     sh_bit_map := (sh_bit_map gps);
+     mod_states := (mod_states gps); |}.
+
+Definition set_gps_shared_bits {Th Tb : Type}
+  (gps : GeneralProgramState Th Tb) (bits : list Tb)
+  : GeneralProgramState Th Tb :=
+  {| sh_hdr_map := (sh_hdr_map gps);
+     sh_bit_map := bits;
+     mod_states := (mod_states gps); |}.
+
+Definition set_gps_mod_states {Th Tb : Type}
+  (gps : GeneralProgramState Th Tb) (ms : PMap.t (ModuleState Th Tb))
+  : GeneralProgramState Th Tb :=
+  {| sh_hdr_map := (sh_hdr_map gps);
+     sh_bit_map := (sh_bit_map gps);
+     mod_states := ms; |}.
+
+Definition GeneralConcreteState : Type := GeneralProgramState CrVal bool.
+Definition GeneralSymbolicState : Type := GeneralProgramState SmtArithExpr SmtBoolExpr.
