HelperLemmas.v
@@ -9,7 +9,7 @@ From MyProject Require Import CrProgramState.
 From MyProject Require Import ListUtils.
 
 Lemma commute_lookup_eval_varlike:
-  forall {A} `{CrVarLike A} (ps : SymbolicState)
+  forall {A} `{CrVarLike A} (ps : SymbolicTransformerState)
         (var : A) (val : SmtValuation),
     lookup_varlike (eval_sym_state ps val) var =
     eval_smt_arith (lookup_varlike ps var) val.
@@ -21,7 +21,7 @@ Proof.
 Qed.
 
 Lemma commute_lookup_eval:
-  forall (s : SymbolicState) (f : SmtValuation)
+  forall (s : SymbolicTransformerState) (f : SmtValuation)
         arg,
     lookup_concrete arg (eval_sym_state s f) =
     eval_smt_arith (lookup_smt arg s) f.
