PMapHelperLemmas.v
@@ -89,43 +89,43 @@ Qed.
 (* lemmas makes them easy to use with `rewrite`.                  *)
 
 Lemma lookup_varlike_header_PMap :
-  forall (s : SymbolicState) (id : positive),
-    lookup_varlike s (HeaderCtr id) = PMap.get id (header_map s).
+  forall (s : SymbolicTransformerState) (id : positive),
+    lookup_varlike s (HeaderCtr id) = PMap.get id (t_header_map s).
 Proof.
   intros. reflexivity.
 Qed.
 
 Lemma lookup_varlike_state_PMap :
-  forall (s : SymbolicState) (id : positive),
-    lookup_varlike s (StateCtr id) = PMap.get id (state_map s).
+  forall (s : SymbolicTransformerState) (id : positive),
+    lookup_varlike s (StateCtr id) = PMap.get id (t_state_map s).
 Proof.
   intros. reflexivity.
 Qed.
 
 Lemma lookup_varlike_ctrl_PMap :
-  forall (s : SymbolicState) (id : positive),
-    lookup_varlike s (CtrlCtr id) = PMap.get id (ctrl_map s).
+  forall (s : SymbolicTransformerState) (id : positive),
+    lookup_varlike s (CtrlCtr id) = PMap.get id (t_ctrl_map s).
 Proof.
   intros. reflexivity.
 Qed.
 
 Lemma lookup_varlike_header_PMap_concrete :
-  forall (s : ConcreteState) (id : positive),
-    lookup_varlike s (HeaderCtr id) = PMap.get id (header_map s).
+  forall (s : ConcreteTransformerState) (id : positive),
+    lookup_varlike s (HeaderCtr id) = PMap.get id (t_header_map s).
 Proof.
   intros. reflexivity.
 Qed.
 
 Lemma lookup_varlike_state_PMap_concrete :
-  forall (s : ConcreteState) (id : positive),
-    lookup_varlike s (StateCtr id) = PMap.get id (state_map s).
+  forall (s : ConcreteTransformerState) (id : positive),
+    lookup_varlike s (StateCtr id) = PMap.get id (t_state_map s).
 Proof.
   intros. reflexivity.
 Qed.
 
 Lemma lookup_varlike_ctrl_PMap_concrete :
-  forall (s : ConcreteState) (id : positive),
-    lookup_varlike s (CtrlCtr id) = PMap.get id (ctrl_map s).
+  forall (s : ConcreteTransformerState) (id : positive),
+    lookup_varlike s (CtrlCtr id) = PMap.get id (t_ctrl_map s).
 Proof.
   intros. reflexivity.
 Qed.
@@ -137,43 +137,43 @@ Qed.
 (* ============================================================ *)
 
 Lemma cs_initialized_in_tree_header :
-  forall (cs : ConcreteState) id w,
-    fst (header_map cs) = (IntVal CrNilInt) ->
-    PMap.get id (header_map cs) = w ->
+  forall (cs : ConcreteTransformerState) id w,
+    fst (t_header_map cs) = (IntVal CrNilInt) ->
+    PMap.get id (t_header_map cs) = w ->
     w <> (IntVal CrNilInt) ->
-    (snd (header_map cs)) ! id = Some w.
+    (snd (t_header_map cs)) ! id = Some w.
 Proof.
   intros cs id w Hdef Heq Hneq.
   unfold PMap.get in Heq.
-  destruct ((snd (header_map cs)) ! id) eqn:Hget.
+  destruct ((snd (t_header_map cs)) ! id) eqn:Hget.
   - subst. reflexivity.
   - subst. contradiction.
 Qed.
 
 Lemma cs_initialized_in_tree_state :
-  forall (cs : ConcreteState) id w,
-    fst (state_map cs) = (IntVal CrNilInt) ->
-    PMap.get id (state_map cs) = w ->
+  forall (cs : ConcreteTransformerState) id w,
+    fst (t_state_map cs) = (IntVal CrNilInt) ->
+    PMap.get id (t_state_map cs) = w ->
     w <> (IntVal CrNilInt) ->
-    (snd (state_map cs)) ! id = Some w.
+    (snd (t_state_map cs)) ! id = Some w.
 Proof.
   intros cs id w Hdef Heq Hneq.
   unfold PMap.get in Heq.
-  destruct ((snd (state_map cs)) ! id) eqn:Hget.
+  destruct ((snd (t_state_map cs)) ! id) eqn:Hget.
   - subst. reflexivity.
   - subst. contradiction.
 Qed.
 
 Lemma cs_initialized_in_tree_ctrl :
-  forall (cs : ConcreteState) id w,
-    fst (ctrl_map cs) = (IntVal CrNilInt) ->
-    PMap.get id (ctrl_map cs) = w ->
+  forall (cs : ConcreteTransformerState) id w,
+    fst (t_ctrl_map cs) = (IntVal CrNilInt) ->
+    PMap.get id (t_ctrl_map cs) = w ->
     w <> (IntVal CrNilInt) ->
-    (snd (ctrl_map cs)) ! id = Some w.
+    (snd (t_ctrl_map cs)) ! id = Some w.
 Proof.
   intros cs id w Hdef Heq Hneq.
   unfold PMap.get in Heq.
-  destruct ((snd (ctrl_map cs)) ! id) eqn:Hget.
+  destruct ((snd (t_ctrl_map cs)) ! id) eqn:Hget.
   - subst. reflexivity.
   - subst. contradiction.
 Qed.
@@ -186,11 +186,11 @@ Lemma init_sym_header_lookup :
   forall hlist slist clist (id : positive),
     Coqlib.list_norepet (List.map (fun (h : Header) => match h with HeaderCtr i => i end) hlist) ->
     In (HeaderCtr id) hlist ->
-    PMap.get id (header_map (init_symbolic_state (CaracaraProgramDef hlist slist clist []))) =
+    PMap.get id (t_header_map (init_symbolic_transformer_state' (CaracaraProgramDef hlist slist clist []))) =
       SmtArithVar ("hdr_" ++ pos_to_string id)%string.
 Proof.
   intros hlist slist clist id Hno Hin.
-  unfold init_symbolic_state, PMap.get. simpl.
+  unfold init_symbolic_transformer_state', PMap.get. simpl.
   set (l := List.map (fun x : Header =>
               let var := match x with HeaderCtr x_id => x_id end in
               (var, SmtArithVar ("hdr_" ++ pos_to_string var))) hlist).
@@ -213,11 +213,11 @@ Lemma init_sym_state_lookup :
   forall hlist slist clist (id : positive),
     Coqlib.list_norepet (List.map (fun (s : State) => match s with StateCtr i => i end) slist) ->
     In (StateCtr id) slist ->
-    PMap.get id (state_map (init_symbolic_state (CaracaraProgramDef hlist slist clist []))) =
+    PMap.get id (t_state_map (init_symbolic_transformer_state' (CaracaraProgramDef hlist slist clist []))) =
       SmtArithVar ("state_" ++ pos_to_string id)%string.
 Proof.
   intros hlist slist clist id Hno Hin.
-  unfold init_symbolic_state, PMap.get. simpl.
+  unfold init_symbolic_transformer_state', PMap.get. simpl.
   set (l := List.map (fun x : State =>
               let var := match x with StateCtr x_id => x_id end in
               (var, SmtArithVar ("state_" ++ pos_to_string var))) slist).
@@ -240,11 +240,11 @@ Lemma init_sym_ctrl_lookup :
   forall hlist slist clist (id : positive),
     Coqlib.list_norepet (List.map (fun (c : Ctrl) => match c with CtrlCtr i => i end) clist) ->
     In (CtrlCtr id) clist ->
-    PMap.get id (ctrl_map (init_symbolic_state (CaracaraProgramDef hlist slist clist []))) =
+    PMap.get id (t_ctrl_map (init_symbolic_transformer_state' (CaracaraProgramDef hlist slist clist []))) =
       SmtArithVar ("ctrl_" ++ pos_to_string id)%string.
 Proof.
   intros hlist slist clist id Hno Hin.
-  unfold init_symbolic_state, PMap.get. simpl.
+  unfold init_symbolic_transformer_state', PMap.get. simpl.
   set (l := List.map (fun x : Ctrl =>
               let var := match x with CtrlCtr x_id => x_id end in
               (var, SmtArithVar ("ctrl_" ++ pos_to_string var))) clist).
@@ -270,10 +270,13 @@ Qed.
 Lemma init_sym_header_lookup_default :
   forall (p : CaracaraProgram) (id : positive),
     ~ In (HeaderCtr id) (get_headers_from_prog p) ->
-    PMap.get id (header_map (init_symbolic_state p)) = SmtArithConst CrNilInt.
+    PMap.get id (t_header_map (init_symbolic_transformer_state' p)) = SmtArithConst CrNilInt.
 Proof.
   intros p id Hnin.
-  unfold init_symbolic_state, PMap.get. cbn [snd fst header_map].
+  unfold init_symbolic_transformer_state',
+         init_symbolic_transformer_state,
+         PMap.get.
+  cbn [snd fst t_header_map].
   match goal with
   | |- match (PTree_Properties.of_list ?L) ! id with _ => _ end = _ =>
       destruct ((PTree_Properties.of_list L) ! id) eqn:Hget; [exfalso | reflexivity];
@@ -286,10 +289,13 @@ Qed.
 Lemma init_sym_state_lookup_default :
   forall (p : CaracaraProgram) (id : positive),
     ~ In (StateCtr id) (get_states_from_prog p) ->
-    PMap.get id (state_map (init_symbolic_state p)) = SmtArithConst CrNilInt.
+    PMap.get id (t_state_map (init_symbolic_transformer_state' p)) = SmtArithConst CrNilInt.
 Proof.
   intros p id Hnin.
-  unfold init_symbolic_state, PMap.get. cbn [snd fst state_map].
+  unfold init_symbolic_transformer_state',
+         init_symbolic_transformer_state,
+         PMap.get.
+  cbn [snd fst t_state_map].
   match goal with
   | |- match (PTree_Properties.of_list ?L) ! id with _ => _ end = _ =>
       destruct ((PTree_Properties.of_list L) ! id) eqn:Hget; [exfalso | reflexivity];
@@ -302,10 +308,13 @@ Qed.
 Lemma init_sym_ctrl_lookup_default :
   forall (p : CaracaraProgram) (id : positive),
     ~ In (CtrlCtr id) (get_ctrls_from_prog p) ->
-    PMap.get id (ctrl_map (init_symbolic_state p)) = SmtArithConst CrNilInt.
+    PMap.get id (t_ctrl_map (init_symbolic_transformer_state' p)) = SmtArithConst CrNilInt.
 Proof.
   intros p id Hnin.
-  unfold init_symbolic_state, PMap.get. cbn [snd fst ctrl_map].
+  unfold init_symbolic_transformer_state',
+         init_symbolic_transformer_state,
+         PMap.get.
+  cbn [snd fst t_ctrl_map].
   match goal with
   | |- match (PTree_Properties.of_list ?L) ! id with _ => _ end = _ =>
       destruct ((PTree_Properties.of_list L) ! id) eqn:Hget; [exfalso | reflexivity];
@@ -323,7 +332,7 @@ Qed.
 (* Cross-type updates do not affect the other map.               *)
 
 Lemma lookup_update_header_header :
-  forall (ps : ConcreteState) (h h' : Header) (x : CrVal),
+  forall (ps : ConcreteTransformerState) (h h' : Header) (x : CrVal),
   lookup_varlike (update_varlike ps h x) h' =
     match h, h' with
     | HeaderCtr hid, HeaderCtr hid' =>
@@ -336,7 +345,7 @@ Proof.
 Qed.
 
 Lemma lookup_update_state_state :
-  forall (ps : ConcreteState) (s s' : State) (x : CrVal),
+  forall (ps : ConcreteTransformerState) (s s' : State) (x : CrVal),
   lookup_varlike (update_varlike ps s x) s' =
     match s, s' with
     | StateCtr sid, StateCtr sid' =>
@@ -349,7 +358,7 @@ Proof.
 Qed.
 
 Lemma lookup_update_ctrl_ctrl :
-  forall (ps : ConcreteState) (c c' : Ctrl) (x : CrVal),
+  forall (ps : ConcreteTransformerState) (c c' : Ctrl) (x : CrVal),
   lookup_varlike (update_varlike ps c x) c' =
     match c, c' with
     | CtrlCtr cid, CtrlCtr cid' =>
